new/proof/math.v
@@ -1,22 +1,25 @@
 From New.generatedproof Require Import math.
 From New.proof Require Import proof_prelude.
 
-Section proof.
-Context  `{hG: heapGS Σ, !ffi_semantics _ _} `{!globalsGS Σ} {go_ctx : GoContext}.
+Section wps.
+Context `{hG: heapGS Σ, !ffi_semantics _ _}.
+Context {sem : go.Semantics} {package_sem : math.Assumptions}.
+Local Set Default Proof Using "All".
 
-#[global] Instance : IsPkgInit math := define_is_pkg_init True%I.
-#[global] Instance : GetIsPkgInitWf math := build_get_is_pkg_init_wf.
+#[global] Instance : IsPkgInit (iProp Σ) math := define_is_pkg_init True%I.
+#[global] Instance : GetIsPkgInitWf (iProp Σ) math := build_get_is_pkg_init_wf.
 
 Lemma wp_initialize' get_is_pkg_init :
   get_is_pkg_init_prop math get_is_pkg_init →
-  {{{ own_initializing get_is_pkg_init ∗ is_go_context ∗ □ is_pkg_defined math }}}
+  {{{ own_initializing get_is_pkg_init }}}
     math.initialize' #()
   {{{ RET #(); own_initializing get_is_pkg_init ∗ is_pkg_init math }}}.
 Proof.
-  intros Hinit. wp_start as "(Hown & #? & #Hdef)".
-  wp_call. wp_apply (wp_package_init with "[$Hown] HΦ").
+  intros Hinit. wp_start as "Hown".
+  wp_apply (wp_package_init with "[$Hown] HΦ").
   { destruct Hinit as (-> & ?); done. }
-  iIntros "Hown". wp_auto. wp_call.
+  iIntros "Hown". wp_auto.
+  iEval (rewrite is_pkg_init_unfold /=). iFrame "∗#".
 Admitted.
 
-End proof.
+End wps.
